CrGeneralProgramState.v
@@ -3,37 +3,85 @@ From MyProject Require Import CrProgramState.
 From MyProject Require Import CrVal.
 From MyProject Require Import SmtExpr.
 
+From Stdlib Require Import List.
+Import ListNotations.
+
 (* [Th] is the header-value type, [Tb] the packet-bit type. *)
 Record GeneralProgramState (Th Tb : Type) := {
   sh_hdr_map : PMap.t Th;
-  sh_bit_map : list Tb;
+  sh_read_tape : list Tb;
+  sh_bits_read : Th;
+  sh_write_tape : list Tb;
   mod_states : PMap.t (ModuleState Th Tb);
+  gps_valid : Tb;
 }.
 
 Arguments sh_hdr_map {Th Tb} _.
-Arguments sh_bit_map {Th Tb} _.
+Arguments sh_read_tape {Th Tb} _.
+Arguments sh_bits_read {Th Tb} _.
+Arguments sh_write_tape {Th Tb} _.
 Arguments mod_states {Th Tb} _.
+Arguments gps_valid {Th Tb} _.
 
 Definition set_gps_shared_headers {Th Tb : Type}
   (gps : GeneralProgramState Th Tb) (hdrs : PMap.t Th)
   : GeneralProgramState Th Tb :=
   {| sh_hdr_map := hdrs;
-     sh_bit_map := (sh_bit_map gps);
-     mod_states := (mod_states gps); |}.
+     sh_read_tape := sh_read_tape gps;
+     sh_bits_read := sh_bits_read gps;
+     sh_write_tape := sh_write_tape gps;
+     mod_states := mod_states gps;
+     gps_valid := gps_valid gps |}.
 
-Definition set_gps_shared_bits {Th Tb : Type}
+Definition set_gps_shared_read_tape {Th Tb : Type}
   (gps : GeneralProgramState Th Tb) (bits : list Tb)
   : GeneralProgramState Th Tb :=
-  {| sh_hdr_map := (sh_hdr_map gps);
-     sh_bit_map := bits;
-     mod_states := (mod_states gps); |}.
+  {| sh_hdr_map := sh_hdr_map gps;
+     sh_read_tape := bits;
+     sh_bits_read := sh_bits_read gps;
+     sh_write_tape := sh_write_tape gps;
+     mod_states := mod_states gps;
+     gps_valid := gps_valid gps |}.
+
+Definition set_gps_bits_read {Th Tb : Type}
+  (gps : GeneralProgramState Th Tb) (n : Th)
+  : GeneralProgramState Th Tb :=
+  {| sh_hdr_map := sh_hdr_map gps;
+     sh_read_tape := sh_read_tape gps;
+     sh_bits_read := n;
+     sh_write_tape := sh_write_tape gps;
+     mod_states := mod_states gps;
+     gps_valid := gps_valid gps |}.
+
+Definition set_gps_shared_write_tape {Th Tb : Type}
+  (gps : GeneralProgramState Th Tb) (cbits : list Tb)
+  : GeneralProgramState Th Tb :=
+  {| sh_hdr_map := sh_hdr_map gps;
+     sh_read_tape := sh_read_tape gps;
+     sh_bits_read := sh_bits_read gps;
+     sh_write_tape := cbits;
+     mod_states := mod_states gps;
+     gps_valid := gps_valid gps |}.
 
 Definition set_gps_mod_states {Th Tb : Type}
   (gps : GeneralProgramState Th Tb) (ms : PMap.t (ModuleState Th Tb))
   : GeneralProgramState Th Tb :=
-  {| sh_hdr_map := (sh_hdr_map gps);
-     sh_bit_map := (sh_bit_map gps);
-     mod_states := ms; |}.
+  {| sh_hdr_map := sh_hdr_map gps;
+     sh_read_tape := sh_read_tape gps;
+     sh_bits_read := sh_bits_read gps;
+     sh_write_tape := sh_write_tape gps;
+     mod_states := ms;
+     gps_valid := gps_valid gps |}.
+
+Definition set_gps_valid {Th Tb : Type}
+  (gps : GeneralProgramState Th Tb) (valid : Tb)
+  : GeneralProgramState Th Tb :=
+  {| sh_hdr_map := sh_hdr_map gps;
+     sh_read_tape := sh_read_tape gps;
+     sh_bits_read := sh_bits_read gps;
+     sh_write_tape := sh_write_tape gps;
+     mod_states := mod_states gps;
+     gps_valid := valid |}.
 
 Definition GeneralConcreteState : Type := GeneralProgramState CrVal bool.
-Definition GeneralSymbolicState : Type := GeneralProgramState SmtArithExpr SmtBoolExpr.
+Definition GeneralSymbolicState : Type := GeneralProgramState SmtArithExpr (ConditionalVal SmtBoolExpr).
